Let $\phi=\frac{1+\sqrt{5}}{2}$ and $\psi=\frac{1-\sqrt{5}}{2}$. We will prove that
$Fib(n) = \frac{\phi^n - \psi^n}{\sqrt{5}}$ using mathematical induction

1. In the base case
$$
\begin{aligned}
Fib (1) &= \frac{\phi - \psi}{\sqrt{5}} \\
& = \frac{\frac{1+\sqrt{5}}{2} - \frac{1-\sqrt{5}}{2}}{\sqrt{5}} \\
& = \frac{1+\sqrt{5}-1+\sqrt{5}}{2\sqrt{5}} \\
& = 1
\end{aligned}
$$

2. Lets assume that $Fib(k) = \frac{\phi^k - \psi^k}{\sqrt{5}}$

3. Consider $Fib(k) + Fib(k-1)$
$$
\begin{aligned}
Fib(k) + Fib(k-1) &=  \frac{\phi^k - \psi^k}{\sqrt{5}} + \frac{\phi^{k-1} - \psi^{k-1}}{\sqrt{5}} \\
& = \frac{1}{\sqrt{5}} (\phi^{k+1}(\frac{1}{\phi} + \frac{1}{\phi^2}) - \psi^{k+1}(\frac{1}{\psi} + \frac{1}{\psi^2}))
\end{aligned}
$$

    We know that $\phi$ and $\psi$ are the roots of the equation $x^2 - x - 1 = 0$, which means
$$
\begin{aligned}
\phi^2 - \phi - 1 &= 0 \\
\phi + 1 & = \phi^2 \\
\frac{1}{\phi} + \frac{1}{\phi^2} & = 1
\end{aligned}
$$

    Similarly $\frac{1}{\psi} + \frac{1}{\psi^2} = 1$. Substituting in the previous equation gives us
$$
\begin{aligned}
Fib(k) + Fib(k-1) &= \frac{1}{\sqrt{5}} (\phi^{k+1} - \psi^{k+1}) \\
& = Fib(k+1)
\end{aligned}
$$

    For larger values of n the second term $\psi^n$ can be ignored. Which gives us
$$
\begin{aligned}
Fib(n) &= \frac{\phi^n}{\sqrt{5}}
\end{aligned}
$$
