Consider the equation
$$
\begin{aligned}
    x &= 1 + \frac{1}{x}
\end{aligned}
$$

Multiplying by x on both sides
$$
\begin{aligned}
    x^2 &= x + 1 \\
    x^2 -x - 1 & = 0
\end{aligned}
$$

This is a quadratic equation whose roots are give by
$$
\begin{aligned}
\frac{-b \pm \sqrt{b^2 - 4ac}}{2a}
\end{aligned}
$$

Substituting the values $a=1, b=-1, c=-1$ we get
$$
\begin{aligned}
    x &= \frac{-(-1) \pm \sqrt{(-1)^2 - 4(1)(-1)}}{2(1)} \\
    x & = \frac{1 \pm \sqrt{5}}{2} \\
    x & = \frac{1 + \sqrt{5}}{2}, \frac{1 - \sqrt{5}}{2} \\
    x & = \phi, \psi
\end{aligned}
$$

To compute the value of $\phi$ all we have to do is

~~~~~ {#mycode .scheme}
(fixed-point (lambda (x) (+ 1 (/ 1 x))) 1.0)

1.6180327868852458
~~~~~
